Todays notes.

04-12-2021.v
@@ -4,29 +4,23 @@ Module IffyLang.
   | T : Exp
   | F : Exp
   | If (b : Exp) (b1 : Exp) (b2 : Exp)
-  | And (b1 : Exp) (b2 : Exp).
+  | And (b1 : Exp) (b2 : Exp).    
 
-   Inductive isVal : Exp -> Prop :=    
-   | valT : isVal T
-   | valF : isVal F.
-
-  Fixpoint  eval (b : Exp) : exists v:Exp, isVal v :=
+  Fixpoint  eval (b : Exp) : Exp :=
     match b with
-    | T => ex_intro isVal T valT
-    | F => ex_intro isVal F valF
+    | T => T
+    | F => F
     | And b1 b2 =>
       match eval b1 with
-      | ex_intro _ F valF => ex_intro isVal F valF
-      | ex_intro _ F valT => _
-      | ex_intro _ T _ => eval b2
-      | ex_intro _ (And b1' b2') _ => ex_intro isVal F valF
-      | ex_intro _ (If b1' b2' b3') _ => ex_intro isVal F valF
+      | T => eval b2
+      | F => F
+      | _ => And b1 b2                           
       end
     | If b' b1 b2 =>
       match eval b' with
-      | ex_intro _ T _ => eval b1
-      | ex_intro _ F _ => eval b2
-      | _ => ex_intro isVal F valF
+      | T => eval b1
+      | F => eval b2
+      | _ => If b' b1 b2
       end
     end.
 
@@ -34,5 +28,54 @@ Module IffyLang.
   Definition exp2 : Exp := If exp1 (And F T) T.
   Compute eval exp2.
 
+  (* Parameterized Data Types *)
+   Inductive isVal' (b : Exp) : Prop :=
+   | valT' : b = T -> isVal' b
+   | valF' : b = F -> isVal' b.
+   
+   (* Indexed Data Types *)
+   Inductive isVal : Exp -> Prop :=    
+   | valT : isVal T
+   | valF : isVal F.   
+
+   Theorem eval_isVal : forall b, isVal (eval b).
+   Proof.
+     intros.
+     induction b.
+
+     - simpl. apply valT.
+     - simpl. apply valF.
+     - simpl. destruct IHb1. apply IHb2. apply IHb3.
+     - simpl. destruct IHb1. apply IHb2. apply valF.
+   Qed.
+
+   (* Intrepret IffyLang into Coq's Prop. Then we will prove
+    * the Coq expression. 
+    * 
+    * => b1 | b2 | b1 -> b2
+    *    T  | T  | T 
+    *    F  | T  | T
+    *    T  | F  | F
+    *    F  | F  | T          *)
+
+   (* The interpretation of IffyLang into Coq. *)
+   Fixpoint toCoq (b : Exp) : Prop :=
+     match b with
+     | T => True
+     | F => False
+     | And b1 b2 => (toCoq b1) /\ (toCoq b2)
+     | If b1 b2 b3 =>
+       ((toCoq b1) -> toCoq b2) /\ (~(toCoq b1) -> toCoq b3)
+     end.
+
+   Theorem eval_sound_T : forall b, eval b = T -> toCoq b.
+   Proof.
+     intros.
+     induction b.
+
+     - simpl. trivial.
+     - simpl. simpl in H. discriminate.
+     - simpl. split. intros. apply IHb2.
+       simpl in H. destruct (eval b1). apply H. 
 End IffyLang.
   
